Phi_System/IDE_CP_Reasoning2.thy
@@ -100,6 +100,8 @@ fn (ctxt, sequent) =>
   end
 \<close>
 
+
+
 (*
 subsection \<open>Extract a Value\<close>
 
